src/Verse/Monoid/Interface.v
@@ -16,12 +16,12 @@ Class Interface {ltypes mtypes}
       (v : Variables.U ltypes)
       (S : mSpecs ltypes mtypes)
   := {
-      Var : forall {k} {ty : typeOf ltypes k},
-        v _ ty -> Variables.Universe.embed (mvariables S)
-                                           (typeTrans (mtypeCompiler S) ty)
+      Var : forall {ty : some (typeOf ltypes)},
+        v ty -> Variables.Universe.embed (mvariables S)
+                                           (Types.Some.translate (mtypeCompiler S) ty)
 
       (* This cannot use Universe.inject as if the typeCompiler
          is a true compiler, a Var map would not be possible at
          all!
        *)
-    }.
+  }.
